GNF.thy
@@ -2,33 +2,33 @@ theory GNF
 imports CFG
 begin
 
-fun nt :: "('n,'t)symbs \<Rightarrow> 'n set" where
+fun nt :: "('n,'t)syms \<Rightarrow> 'n set" where
 "nt [] = {}" |
-"nt (N A # v) = {A} \<union> nt v" |
-"nt (T a # v) = nt v"
+"nt (NT A # v) = {A} \<union> nt v" |
+"nt (Tm a # v) = nt v"
 
-lemma nt_Cons: "nt (a#v) = (case a of N A \<Rightarrow> {A} | _ \<Rightarrow> {}) \<union> nt v"
+lemma nt_Cons: "nt (a#v) = (case a of NT A \<Rightarrow> {A} | _ \<Rightarrow> {}) \<union> nt v"
   by (cases a, auto)
 
 lemma nt_append[simp]: "nt (u @ v) = nt u \<union> nt v"
   apply (induction u arbitrary: v rule: nt.induct)
   by auto
 
-fun rt :: "('n,'t)symbs \<Rightarrow> bool" where
+fun rt :: "('n,'t)syms \<Rightarrow> bool" where
 "rt [] = True" |
-"rt (T _ # _) = True" |
+"rt (Tm _ # _) = True" |
 "rt _ = False"
 
 definition rtps :: "('n,'t)prods \<Rightarrow> bool" where
 "rtps ps = (\<forall>p \<in> ps. rt(snd p))"
 
-definition Lnt :: "('n, 't) prods \<Rightarrow> ('n * 'n * ('n,'t)symbs)set" where
-"Lnt P = {(A,B,w). (A, N B # w) \<in> P}"
+definition Lnt :: "('n, 't) prods \<Rightarrow> ('n * 'n * ('n,'t)syms)set" where
+"Lnt P = {(A,B,w). (A, NT B # w) \<in> P}"
 
-lemma [code]: "Lnt P = \<Union> ((\<lambda>(A,w). case w of N B#v \<Rightarrow> {(A,B,v)} | _ \<Rightarrow> {}) ` P)"
-  by (auto simp: Lnt_def split: list.splits symb.splits)
+lemma [code]: "Lnt P = \<Union> ((\<lambda>(A,w). case w of NT B#v \<Rightarrow> {(A,B,v)} | _ \<Rightarrow> {}) ` P)"
+  by (auto simp: Lnt_def split: list.splits sym.splits)
 
-definition rule where "rule = (\<lambda>(A, B, w). (A, N B # w))"
+definition rule where "rule = (\<lambda>(A, B, w). (A, NT B # w))"
 
 lemma Lnt_Un: "Lnt (A \<union> B) = Lnt A \<union> Lnt B"
 by(auto simp: Lnt_def)
@@ -41,10 +41,10 @@ by(auto simp: Lnt_def rule_def image_def split:prod.splits)
 
 (*
 fun lnt :: "('n,'t)prod \<Rightarrow> 'n option" where
-"lnt(_,N A # _) = Some A" |
+"lnt(_,NT A # _) = Some A" |
 "lnt _ = None"
 
-definition "has_lnt p = (\<exists>A u. snd p = N A # u)"
+definition "has_lnt p = (\<exists>A u. snd p = NT A # u)"
 
 lemma has_lnt_iff_lnt_split_Some: "has_lnt p = (\<exists>A. lnt_split p = Some A)"
 by(cases p rule: lnt_split.cases) (auto simp: has_lnt_def)
@@ -82,7 +82,7 @@ definition "Rhs1 R = rhs1 ` Lnt R"
 lemma lem: "A - {x. P x} = {x\<in>A. \<not>P x}"
 by auto
 
-lemma Rhs1_subsetD: "Rhs1 R \<subseteq> M \<Longrightarrow> (A, N B # w) \<in> R \<Longrightarrow> B \<in> M"
+lemma Rhs1_subsetD: "Rhs1 R \<subseteq> M \<Longrightarrow> (A, NT B # w) \<in> R \<Longrightarrow> B \<in> M"
 sorry
 
 lemma Lnt_subset: "R \<subseteq> S \<Longrightarrow> Lnt R \<subseteq> Lnt S"
@@ -94,21 +94,21 @@ lemma Rhs1_subset: "R \<subseteq> S \<Longrightarrow> Rhs1 R \<subseteq> Rhs1 S"
 lemma Rhs1_Un: "Rhs1 (R \<union> S) = Rhs1 R \<union> Rhs1 S"
   by (auto simp: Rhs1_def Lnt_def)
 
-fun starts_with where "starts_with A (N B # w) \<longleftrightarrow> A = B"
+fun starts_with where "starts_with A (NT B # w) \<longleftrightarrow> A = B"
   | "starts_with _ _ = False"
 
-lemma starts_with_iff: "starts_with A w \<longleftrightarrow> (\<exists>v. w = N A # v)"
+lemma starts_with_iff: "starts_with A w \<longleftrightarrow> (\<exists>v. w = NT A # v)"
   apply (cases "(A,w)" rule: starts_with.cases) by auto
 
-definition "ends_with A w = (\<exists>v. w = v @ [N A])"
+definition "ends_with A w = (\<exists>v. w = v @ [NT A])"
 
 lemma ends_with_iff_starts_with_rev: "ends_with A w \<longleftrightarrow> starts_with A (rev w)"
   apply (auto simp: starts_with_iff ends_with_def)
   by (metis rev_rev_ident)
 
-definition "loop R A = {(A,N A # w) | w. (A, N A # w) \<in> R \<and> w \<noteq> []}"
+definition "loop R A = {(A,NT A # w) | w. (A, NT A # w) \<in> R \<and> w \<noteq> []}"
 
-definition "right_loop R A = {(A,w@[N A]) | w. (A, w@[N A]) \<in> R \<and> w \<noteq> []}"
+definition "right_loop R A = {(A,w@[NT A]) | w. (A, w@[NT A]) \<in> R \<and> w \<noteq> []}"
 
 lemma right_loop_eq_loop:
   "right_loop R A = map_prod id rev ` loop (map_prod id rev ` R) A"
@@ -120,7 +120,7 @@ lemma loop_freeI:
   assumes "\<And>w. (A,w) \<in> R \<Longrightarrow> \<not>starts_with A w" shows "loop_free R A"
   using assms by (auto simp: loop_free_def)
 
-lemma loop_freeD: "loop_free R A \<Longrightarrow> (A, N A # w) \<notin> R"
+lemma loop_freeD: "loop_free R A \<Longrightarrow> (A, NT A # w) \<notin> R"
   by (auto simp: loop_free_def)
 
 definition "loop_free_list R A = (\<forall>(B,w) \<in> set R. B = A \<longrightarrow> \<not> starts_with A w)"
@@ -143,16 +143,16 @@ lemma solved: "solved (set R) (set As) = solved_list R As"
   by (auto simp: solved_def solved_list_def)
 
 lemma solved_not:
-  "solved R As \<Longrightarrow> A \<in> As \<Longrightarrow> (B,N A#w) \<notin> R"
+  "solved R As \<Longrightarrow> A \<in> As \<Longrightarrow> (B,NT A#w) \<notin> R"
   apply (auto simp: solved_def split: prod.splits)
   by (metis starts_with.simps(1))
 
-definition Nts where "Nts R = concat [A#[B. N B \<leftarrow> w]. (A,w) \<leftarrow> R]"
+definition Nts where "Nts R = concat [A#[B. NT B \<leftarrow> w]. (A,w) \<leftarrow> R]"
 
-definition Nt where "Nt R = (\<Union>(A,w)\<in>R. {A}\<union>{B. N B \<in> set w})"
+definition Nt where "Nt R = (\<Union>(A,w)\<in>R. {A}\<union>{B. NT B \<in> set w})"
 
 fun hdnt where
-    "hdnt (N A#w) = Some A"
+    "hdnt (NT A#w) = Some A"
   | "hdnt _ = None"
 
 lemma set_Nts_def: "set (Nts R) = Nt (set R)"
@@ -172,11 +172,11 @@ qed
 
 definition unwind_new where
   "unwind_new R A A' = (
-  \<Union>{{(A',w), (A',w@[N A'])} | w. (A,N A # w) \<in> R \<and> w \<noteq> []})"
+  \<Union>{{(A',w), (A',w@[NT A'])} | w. (A,NT A # w) \<in> R \<and> w \<noteq> []})"
 
 definition unwind_new_list where
   "unwind_new_list R A A' =
-  concat [[(A',w), (A',w@[N A'])]. (B,N C # w) \<leftarrow> R, B = A \<and> C = A \<and> w \<noteq> []]"
+  concat [[(A',w), (A',w@[NT A'])]. (B,NT C # w) \<leftarrow> R, B = A \<and> C = A \<and> w \<noteq> []]"
 
 lemma set_unwind_new_list: "set (unwind_new_list R A A') = unwind_new (set R) A A'"
   apply (auto simp: unwind_new_list_def unwind_new_def starts_with_iff)
@@ -185,14 +185,14 @@ lemma set_unwind_new_list: "set (unwind_new_list R A A') = unwind_new (set R) A 
 
 definition unwind_old where
   "unwind_old R A A' = (
-  let X = {(A, N A # w) | w. (A, N A # w) \<in> R} in
-  R - X \<union> {(A, w@[N A']) |w. (A,w) \<in> R - X})"
+  let X = {(A, NT A # w) | w. (A, NT A # w) \<in> R} in
+  R - X \<union> {(A, w@[NT A']) |w. (A,w) \<in> R - X})"
 
 definition unwind_old_list where
   "unwind_old_list R A A' = (
   let X = [(B,w) \<leftarrow> R. B = A \<and> starts_with A w] in
   diff_list X R @
-  [(A, w@[N A']). (B,w) \<leftarrow> R, B = A \<and> \<not> starts_with A w])"
+  [(A, w@[NT A']). (B,w) \<leftarrow> R, B = A \<and> \<not> starts_with A w])"
 
 lemma set_unwind_old_list: "set (unwind_old_list R A A') = unwind_old (set R) A A'"
   by (auto simp: unwind_old_def unwind_old_list_def starts_with_iff)
@@ -213,34 +213,34 @@ definition unwind_old_expand_list where
   "unwind_old_expand_list R A A' = (
   let X = [(B,w) \<leftarrow> R. starts_with A w] in
   diff_list X R @
-  [(A, w@[N A']). (B,w) \<leftarrow> R, B = A \<and> \<not> starts_with A w] @
-  concat [[(B,w@tl v),(B,w@N A'#tl v)]. (B,v) \<leftarrow> R, (C,w) \<leftarrow> diff_list X R, starts_with A v \<and> A \<noteq> B \<and> C = A ])"
+  [(A, w@[NT A']). (B,w) \<leftarrow> R, B = A \<and> \<not> starts_with A w] @
+  concat [[(B,w@tl v),(B,w@NT A'#tl v)]. (B,v) \<leftarrow> R, (C,w) \<leftarrow> diff_list X R, starts_with A v \<and> A \<noteq> B \<and> C = A ])"
 
 definition unwind_old_expand where
   "unwind_old_expand R A A' = (
-  let X = {(B, N A # w) | B w. (B, N A # w) \<in> R} in
-  R - X \<union> {(A, w @ [N A']) |w. (A,w) \<in> R - X} \<union>
-  \<Union>{{(B, w@v), (B, w @ N A' # v)} |B v w.
- (B, N A # v) \<in> R \<and> A \<noteq> B \<and> (A,w) \<in> R - X })"
+  let X = {(B, NT A # w) | B w. (B, NT A # w) \<in> R} in
+  R - X \<union> {(A, w @ [NT A']) |w. (A,w) \<in> R - X} \<union>
+  \<Union>{{(B, w@v), (B, w @ NT A' # v)} |B v w.
+ (B, NT A # v) \<in> R \<and> A \<noteq> B \<and> (A,w) \<in> R - X })"
 
 lemma set_unwind_old_expand_list: "set (unwind_old_expand_list R A A') = unwind_old_expand (set R) A A'"
   apply (auto simp: unwind_old_expand_def unwind_old_expand_list_def starts_with_iff)
   sorry
 
 definition "expand R S As =
-  {(A, b # w) |A b w. (A, b # w) \<in> R \<and> b \<notin> N ` As} \<union>
-  {(A,v@w) |A v w. \<exists>B \<in> As. (A,N B # w) \<in> R \<and> (B,v) \<in> S}"
+  {(A, b # w) |A b w. (A, b # w) \<in> R \<and> b \<notin> NT ` As} \<union>
+  {(A,v@w) |A v w. \<exists>B \<in> As. (A,NT B # w) \<in> R \<and> (B,v) \<in> S}"
 
 lemma derive_expand_iff:
   shows "expand R S As \<turnstile> u \<Rightarrow> v \<longleftrightarrow>
-  (\<exists>u1 u2 A b w. (A, b # w) \<in> R \<and> u = u1 @ N A # u2 \<and>
-  (b \<notin> N ` As \<and> v = u1 @ b # w @ u2 \<or>
-  (\<exists>(C,r) \<in> S. C \<in> As \<and> b = N C \<and> v = u1 @ r @ w @ u2)))"
+  (\<exists>u1 u2 A b w. (A, b # w) \<in> R \<and> u = u1 @ NT A # u2 \<and>
+  (b \<notin> NT ` As \<and> v = u1 @ b # w @ u2 \<or>
+  (\<exists>(C,r) \<in> S. C \<in> As \<and> b = NT C \<and> v = u1 @ r @ w @ u2)))"
   by (fastforce simp: Bex_def expand_def derive_iff split:prod.splits)
 
 definition "expand_list R S As =
-  [(A, b # w). (A, b # w) \<leftarrow> R, b \<notin> N ` set As] @
-  [(A,v@w). (A, N B # w) \<leftarrow> R, B \<in> set As, (C,v) \<leftarrow> S, C = B]"
+  [(A, b # w). (A, b # w) \<leftarrow> R, b \<notin> NT ` set As] @
+  [(A,v@w). (A, NT B # w) \<leftarrow> R, B \<in> set As, (C,v) \<leftarrow> S, C = B]"
 
 lemma set_expand_list: "set (expand_list R S As) = expand (set R) (set S) (set As)"
   by (auto simp: expand_list_def expand_def)
@@ -273,8 +273,8 @@ lemma unwind_old_expand:
            apply (auto; blast)[]
           apply (auto; blast)[]
          apply (auto)[]
-         apply (metis append_eq_Cons_conv list.inject symb.inject(2))
-        apply (metis (no_types, lifting) Cons_eq_append_conv list.inject symb.inject(2))
+         apply (metis append_eq_Cons_conv list.inject sym.inject(1))
+        apply (metis (no_types, lifting) Cons_eq_append_conv list.inject sym.inject(1))
        apply blast
       apply blast
      apply (metis (mono_tags, lifting) Cons_eq_appendI append_assoc eps_freeE_Cons list.inject)
@@ -327,9 +327,9 @@ definition "unwind_expand'_list R As A A' = (
   let R' = unwind_list R A A' in
   expand_list R' R' (A#As))"
 
-value "unwind_old_expand_list [(2, [N 1::(int,int)symb])] 1 2"
+value "unwind_old_expand_list [(2, [NT 1::(int,int)sym])] 1 2"
 
-value "solved_list [(2::int, [N 2::(int,int)symb, N 1]), (1, [N 2])] [1]"
+value "solved_list [(2::int, [NT 2::(int,int)sym, NT 1]), (1, [NT 2])] [1]"
 
 lemma expand_derives_imp:
   assumes ef: "eps_free R"
@@ -349,13 +349,13 @@ next
      apply (rule r_into_rtranclp)
     using derive.intros Un_derive apply fastforce
     subgoal premises Aw  for u1 u2 A w B v
-      apply (rule rtranclp_trans[of _ _ "u1@N B # w@u2",OF r_into_rtranclp r_into_rtranclp])
+      apply (rule rtranclp_trans[of _ _ "u1@NT B # w@u2",OF r_into_rtranclp r_into_rtranclp])
       using Aw Un_derive derive.intros apply fastforce
     proof-
       from Aw
-      have "S \<turnstile> u1 @ N B # w @ u2 \<Rightarrow> u1 @ v @ w @ u2"
+      have "S \<turnstile> u1 @ NT B # w @ u2 \<Rightarrow> u1 @ v @ w @ u2"
         using derive.simps by fastforce
-      with Aw(1-5) show "R \<union> S \<turnstile> u1 @ N B # w @ u2 \<Rightarrow> u1 @ v @ w @ u2"
+      with Aw(1-5) show "R \<union> S \<turnstile> u1 @ NT B # w @ u2 \<Rightarrow> u1 @ v @ w @ u2"
         using Un_derive ef eps_freeE_Cons by fastforce
     qed
     done
@@ -365,11 +365,11 @@ qed
 lemma expand_derivels:
   assumes ef: "eps_free R"
     and RAs: "fst ` R \<inter> As = {}"
-    and der: "R \<union> S \<turnstile> u \<Rightarrow>l* map T v"
-  shows "expand R S As \<union> S \<turnstile> u \<Rightarrow>l* map T v"
+    and der: "R \<union> S \<turnstile> u \<Rightarrow>l* map Tm v"
+  shows "expand R S As \<union> S \<turnstile> u \<Rightarrow>l* map Tm v"
 proof-
   from der
-  obtain n where "R \<union> S \<turnstile> u \<Rightarrow>l(n) map T v"
+  obtain n where "R \<union> S \<turnstile> u \<Rightarrow>l(n) map Tm v"
     by (metis rtranclp_imp_relpowp)
   then show ?thesis
   proof (induction n arbitrary: u rule: less_induct)
@@ -380,7 +380,7 @@ proof-
       then show ?thesis using less.prems by auto
     next
       case [simp]: (Suc m)
-      then obtain z where uz: "R \<union> S \<turnstile> u \<Rightarrow>l z" and zv: "R \<union> S \<turnstile> z \<Rightarrow>l(m) map T v"
+      then obtain z where uz: "R \<union> S \<turnstile> u \<Rightarrow>l z" and zv: "R \<union> S \<turnstile> z \<Rightarrow>l(m) map Tm v"
         by (metis less.prems relpowp_Suc_E2)
       from uz have "R \<turnstile> u \<Rightarrow>l z \<or> (S \<turnstile> u \<Rightarrow>l z)"
         by (simp add: Un_derivel)
@@ -391,27 +391,27 @@ proof-
           by (metis Suc Un_derivel zv converse_rtranclp_into_rtranclp less.IH lessI)
       next
         assume "R \<turnstile> u \<Rightarrow>l z"
-        then obtain p A w y2 where [simp]: "u = map T p @ N A # y2"
+        then obtain p A w y2 where [simp]: "u = map Tm p @ NT A # y2"
           and Aw: "(A,w) \<in> R"
-          and [simp]:"z = map T p @ w @ y2"
+          and [simp]:"z = map Tm p @ w @ y2"
           by (meson derivel.cases)
         with ef obtain a w2 where [simp]: "w = a # w2" by (auto dest: eps_freeE_Cons)
         show ?thesis
-        proof (cases "a \<in> N ` As")
+        proof (cases "a \<in> NT ` As")
           case True
-          then obtain B where [simp]: "a = N B" and B: "B \<in> As" by auto
+          then obtain B where [simp]: "a = NT B" and B: "B \<in> As" by auto
           from zv have "m \<noteq> 0"
             apply (intro notI)
-            by (auto simp: deriveln_map_T_append Cons_eq_map_conv append_eq_map_conv)
+            by (auto simp: deriveln_map_Tm_append Cons_eq_map_conv append_eq_map_conv)
           then obtain l where [simp]: "m = Suc l"
             using old.nat.exhaust by auto
           from zv obtain z' where zz': "R \<union> S \<turnstile> z \<Rightarrow>l z'"
-            and z'v: "R \<union> S \<turnstile> z' \<Rightarrow>l(l) map T v"
+            and z'v: "R \<union> S \<turnstile> z' \<Rightarrow>l(l) map Tm v"
             by (metis \<open>m = Suc l\<close> relpowp_Suc_D2)
-          from zz' have "\<exists>y. (B,y) \<in> R \<union> S \<and> z' = map T p @ y @ w2 @ y2"
+          from zz' have "\<exists>y. (B,y) \<in> R \<union> S \<and> z' = map Tm p @ y @ w2 @ y2"
             by (auto simp:derivel_iff append_eq_append_conv2 map_eq_append_conv append_eq_map_conv append_eq_Cons_conv Cons_eq_append_conv)
           then obtain y where By: "(B,y) \<in> R \<union> S"
-            and [simp]: "z' = map T p @ y @ w2 @ y2" by auto
+            and [simp]: "z' = map Tm p @ y @ w2 @ y2" by auto
           with B RAs have "(B,y) \<in> S" by auto
           with Aw B
           have "(A,y@w2) \<in> expand R S As" by (auto simp: expand_def)
@@ -419,7 +419,7 @@ proof-
             using derivel.intros by fastforce
           then have "expand R S As \<union> S \<turnstile> u \<Rightarrow>l z'" by (auto simp: Un_derivel)
           also from less.IH[OF _ z'v]
-          have "expand R S As \<union> S \<turnstile> z' \<Rightarrow>l* map T v" by auto
+          have "expand R S As \<union> S \<turnstile> z' \<Rightarrow>l* map Tm v" by auto
           finally show ?thesis by auto
         next
           case False
@@ -440,7 +440,7 @@ qed
 lemma expand_derives:
   assumes ef: "eps_free R"
     and RAs: "fst ` R \<inter> As = {}"
-  shows "expand R S As \<union> S \<turnstile> u \<Rightarrow>* map T v \<longleftrightarrow> R \<union> S \<turnstile> u \<Rightarrow>* map T v"
+  shows "expand R S As \<union> S \<turnstile> u \<Rightarrow>* map Tm v \<longleftrightarrow> R \<union> S \<turnstile> u \<Rightarrow>* map Tm v"
   using expand_derives_imp[OF ef]
     expand_derivels[unfolded derivels_iff_derives, OF ef RAs]
   by auto
@@ -464,14 +464,14 @@ lemma eps_free_unwind_new: "eps_free (unwind_new R A A')"
   sorry
 
 lemma in_loop: "(B, w) \<in> loop R A \<longleftrightarrow>
-  A = B \<and> (A,w) \<in> R \<and> (\<exists>w'. w = N A # w' \<and> w' \<noteq> [])"
+  A = B \<and> (A,w) \<in> R \<and> (\<exists>w'. w = NT A # w' \<and> w' \<noteq> [])"
   by (auto simp: loop_def)
 
 lemma extract_loop:
-  assumes "R \<turnstile> N A # u \<Rightarrow>l(n) v" and vA: "\<not>starts_with A v"
+  assumes "R \<turnstile> NT A # u \<Rightarrow>l(n) v" and vA: "\<not>starts_with A v"
   shows "\<exists>n1 n2 u' w.
     n1 + n2 < n \<and>
-    loop R A \<turnstile> [N A] \<Rightarrow>l(n1) N A # u' \<and>
+    loop R A \<turnstile> [NT A] \<Rightarrow>l(n1) NT A # u' \<and>
     (A,w) \<in> R \<and> \<not>starts_with A w \<and> R \<turnstile> w@u'@u \<Rightarrow>l(n2) v"
   using assms(1)
 proof (induction n arbitrary: u)
@@ -481,14 +481,14 @@ next
   case (Suc n)
   from Suc.prems
   obtain w where Aw: "(A,w) \<in> R" and wuv: "R \<turnstile> w@u \<Rightarrow>l(n) v"
-    by (auto simp: relpowp_Suc_left derivel_N_Cons)
+    by (auto simp: relpowp_Suc_left derivel_NT_Cons)
   show ?case
   proof (cases "starts_with A w")
     case True
-    then obtain w' where [simp]: "w = N A # w'" by (auto simp: starts_with_iff)
+    then obtain w' where [simp]: "w = NT A # w'" by (auto simp: starts_with_iff)
     from Suc.IH[OF wuv[simplified]]
     obtain n1 n2 u' x where len: "n1 + n2 < n"
-      and n1: "loop R A \<turnstile> [N A] \<Rightarrow>l(n1) N A # u'"
+      and n1: "loop R A \<turnstile> [NT A] \<Rightarrow>l(n1) NT A # u'"
       and AxR: "(A, x) \<in> R"
       and Ax: "\<not> starts_with A x"
       and n2: "R \<turnstile> x @ u' @ w' @ u \<Rightarrow>l(n2) v"
@@ -500,9 +500,9 @@ next
     next
       case w': False
       from w' Aw have "(A,w) \<in> loop R A" by (auto simp: in_loop)
-      then have "loop R A \<turnstile> [N A] \<Rightarrow>l N A # w'" by (auto simp: derivel_N_Cons)
+      then have "loop R A \<turnstile> [NT A] \<Rightarrow>l NT A # w'" by (auto simp: derivel_NT_Cons)
       also from deriveln_append[OF n1, of w']
-      have "loop R A \<turnstile> \<dots> \<Rightarrow>l(n1) N A # u' @ w'" by simp
+      have "loop R A \<turnstile> \<dots> \<Rightarrow>l(n1) NT A # u' @ w'" by simp
       finally show ?thesis using len AxR Ax n2 by force
     qed
   next
@@ -513,10 +513,10 @@ next
 qed
 
 lemma extract_right_loop:
-  assumes "R \<turnstile> u @ [N A] \<Rightarrow>r(n) v" and vA: "\<not>ends_with A v"
+  assumes "R \<turnstile> u @ [NT A] \<Rightarrow>r(n) v" and vA: "\<not>ends_with A v"
   shows "\<exists>n1 n2 u' w.
     n1 + n2 < n \<and>
-    right_loop R A \<turnstile> [N A] \<Rightarrow>r(n1) u' @ [N A] \<and>
+    right_loop R A \<turnstile> [NT A] \<Rightarrow>r(n1) u' @ [NT A] \<and>
     (A,w) \<in> R \<and> \<not>ends_with A w \<and> R \<turnstile> u@u'@w \<Rightarrow>r(n2) v"
 proof-
   from extract_loop[of n "map_prod id rev ` R" A "rev u" "rev v"] assms
@@ -531,10 +531,10 @@ proof-
 qed
 
 lemma unwind_new_simulate_loop:
-  assumes "loop R A \<turnstile> [N A] \<Rightarrow>l+ N A # vs"
-  shows "unwind_new R A A' \<turnstile> [N A'] \<Rightarrow>* vs"
+  assumes "loop R A \<turnstile> [NT A] \<Rightarrow>l+ NT A # vs"
+  shows "unwind_new R A A' \<turnstile> [NT A'] \<Rightarrow>* vs"
   using assms
-proof (induction "N A # vs" arbitrary: vs rule: tranclp_induct)
+proof (induction "NT A # vs" arbitrary: vs rule: tranclp_induct)
   case base
   then show ?case
     apply (intro conjI r_into_rtranclp)
@@ -542,16 +542,16 @@ proof (induction "N A # vs" arbitrary: vs rule: tranclp_induct)
         derive_singleton)
 next
   case (step y z)
-  then obtain y' where [simp]: "y = N A # y'"
+  then obtain y' where [simp]: "y = NT A # y'"
     by (auto simp: derivel_iff in_loop Cons_eq_append_conv)
   from step[simplified]
-  have IH: "unwind_new R A A' \<turnstile> [N A'] \<Rightarrow>* y'" by auto
-  obtain v where AAv: "(A,N A # v) \<in> R"
+  have IH: "unwind_new R A A' \<turnstile> [NT A'] \<Rightarrow>* y'" by auto
+  obtain v where AAv: "(A,NT A # v) \<in> R"
     and [simp]: "z = v @ y'"
     and v0: "v \<noteq> []"
     using step(2)
     by (auto simp: derivel_iff Cons_eq_append_conv in_loop)
-  from v0 have "(A', v @ [N A']) \<in> unwind_new R A A'"
+  from v0 have "(A', v @ [NT A']) \<in> unwind_new R A A'"
       using AAv by (auto simp: unwind_new_def)
   with IH show ?case apply auto
     by (meson converse_rtranclp_into_rtranclp derive_singleton derives_prepend)
@@ -559,8 +559,8 @@ qed
 
 (*AY: could be generalized so that A is not left-most nonterminal of v. *)
 lemma unwind_complete:
-  assumes "R \<turnstile> u \<Rightarrow>l(n) map T v"
-  shows "unwind R A A' \<turnstile> u \<Rightarrow>* map T v"
+  assumes "R \<turnstile> u \<Rightarrow>l(n) map Tm v"
+  shows "unwind R A A' \<turnstile> u \<Rightarrow>* map Tm v"
   using assms
 proof (induction n arbitrary: u v rule: less_induct)
   case (less n)
@@ -571,62 +571,62 @@ proof (induction n arbitrary: u v rule: less_induct)
   next
     case [simp]: (Suc m)
     with less.prems obtain p B w u' v' where Bw: "(B,w) \<in> R"
-      and [simp]: "u = map T p @ N B # u'" "v = p @ v'"
-      and m: "R \<turnstile> w @ u' \<Rightarrow>l(m) map T v'"
+      and [simp]: "u = map Tm p @ NT B # u'" "v = p @ v'"
+      and m: "R \<turnstile> w @ u' \<Rightarrow>l(m) map Tm v'"
       apply (auto simp: relpowp_Suc_left derivel_iff[of R u] Cons_eq_append_conv append_eq_Cons_conv
           split: prod.splits)
-      by (smt (z3) append_eq_map_conv deriveln_map_T_append)
+      by (smt (z3) append_eq_map_conv deriveln_map_Tm_append)
     show ?thesis
     proof (cases "B = A")
       case [simp]: True
-      have "R \<turnstile> N A # u' \<Rightarrow>l w @ u'" using Bw
-        by (auto simp: derivel_N_Cons)
+      have "R \<turnstile> NT A # u' \<Rightarrow>l w @ u'" using Bw
+        by (auto simp: derivel_NT_Cons)
       also note m
-      finally have "R \<turnstile> N A # u' \<Rightarrow>l(n) map T v'" by simp
+      finally have "R \<turnstile> NT A # u' \<Rightarrow>l(n) map Tm v'" by simp
       from extract_loop[OF this]
       obtain n1 n2 u'' w'
         where len: "n1 + n2 < n"
-          and n1: "loop R A \<turnstile> [N A] \<Rightarrow>l(n1) N A # u''"
+          and n1: "loop R A \<turnstile> [NT A] \<Rightarrow>l(n1) NT A # u''"
           and Aw'R: "(A, w') \<in> R"
           and Aw': "\<not> starts_with A w'"
-          and n2: "R \<turnstile> w' @ u'' @ u' \<Rightarrow>l(n2) map T v'" by (fastforce simp: starts_with_iff)
+          and n2: "R \<turnstile> w' @ u'' @ u' \<Rightarrow>l(n2) map Tm v'" by (fastforce simp: starts_with_iff)
       from less.IH[OF _ n2] len
-      have IH: "unwind R A A' \<turnstile> w' @ u'' @ u' \<Rightarrow>* map T v'" by auto
+      have IH: "unwind R A A' \<turnstile> w' @ u'' @ u' \<Rightarrow>* map Tm v'" by auto
       show ?thesis
       proof (cases "n1 > 0")
         case True
-        from Aw' Aw'R have "(A,w'@[N A']) \<in> unwind R A A'"
+        from Aw' Aw'R have "(A,w'@[NT A']) \<in> unwind R A A'"
           by (auto simp: unwind_def unwind_old_def)
-        then have "unwind R A A' \<turnstile> u \<Rightarrow> map T p @ w' @ N A' # u'"
+        then have "unwind R A A' \<turnstile> u \<Rightarrow> map Tm p @ w' @ NT A' # u'"
           by (force simp: derive_iff)
-        also have "unwind R A A' \<turnstile> \<dots> \<Rightarrow>* map T p @ w' @ u'' @ u'"
+        also have "unwind R A A' \<turnstile> \<dots> \<Rightarrow>* map Tm p @ w' @ u'' @ u'"
         proof (intro derives_prepend)
-          from True n1 have "loop R A \<turnstile> [N A] \<Rightarrow>l+ N A # u''"
+          from True n1 have "loop R A \<turnstile> [NT A] \<Rightarrow>l+ NT A # u''"
             by (metis tranclp_power)
           from unwind_new_simulate_loop[OF this, of A']
-          have "unwind R A A' \<turnstile> [N A'] \<Rightarrow>* u''"
+          have "unwind R A A' \<turnstile> [NT A'] \<Rightarrow>* u''"
             by (metis Un_derive mono_rtranclp unwind_def)
           from derives_append[OF this]
-          show "unwind R A A' \<turnstile> N A' # u' \<Rightarrow>* u'' @ u'" by simp
+          show "unwind R A A' \<turnstile> NT A' # u' \<Rightarrow>* u'' @ u'" by simp
         qed
-        also have "unwind R A A' \<turnstile> \<dots> \<Rightarrow>* map T v"
+        also have "unwind R A A' \<turnstile> \<dots> \<Rightarrow>* map Tm v"
           by (simp add: IH derives_prepend)
         finally show ?thesis.
       next
         case False
-        from Aw'R Aw' have "unwind R A A' \<turnstile> N A # u' \<Rightarrow> w' @ u'"
-          by (auto intro!: derivel_imp_derive simp: derivel_N_Cons unwind_def unwind_old_def)
+        from Aw'R Aw' have "unwind R A A' \<turnstile> NT A # u' \<Rightarrow> w' @ u'"
+          by (auto intro!: derivel_imp_derive simp: derivel_NT_Cons unwind_def unwind_old_def)
         with n1 IH False show ?thesis by (auto intro!:derives_prepend)
       qed
     next
       case False
       with Bw have "(B,w) \<in> unwind_old R A A'"
         by (auto simp: unwind_old_def)
-      then have "unwind R A A' \<turnstile> u \<Rightarrow> map T p @ w @ u'"
+      then have "unwind R A A' \<turnstile> u \<Rightarrow> map Tm p @ w @ u'"
         by (auto simp: derive_iff unwind_def)
       also from less.IH[OF _ m]
-      have "unwind R A A' \<turnstile> w @ u' \<Rightarrow>* map T v'" by auto
-      then have "unwind R A A' \<turnstile> map T p @ w @ u' \<Rightarrow>* map T v"
+      have "unwind R A A' \<turnstile> w @ u' \<Rightarrow>* map Tm v'" by auto
+      then have "unwind R A A' \<turnstile> map Tm p @ w @ u' \<Rightarrow>* map Tm v"
         using derives_prepend by auto
       finally show ?thesis.
     qed
@@ -634,7 +634,7 @@ proof (induction n arbitrary: u v rule: less_induct)
 qed
 
 lemma derive_Cons_undef:
-  assumes "a \<notin> N ` fst ` R"
+  assumes "a \<notin> NT ` fst ` R"
   shows "R \<turnstile> a # u \<Rightarrow> v \<longleftrightarrow> (\<exists>v'. v = a # v' \<and> R \<turnstile> u \<Rightarrow> v')"
   using assms
   apply (auto simp: derive_iff Cons_eq_append_conv split:prod.splits)
@@ -651,7 +651,7 @@ proof (induction p arbitrary: u v)
   then show ?case by auto
 next
   case (Cons a p)
-  then have "a \<notin> N ` fst ` R"
+  then have "a \<notin> NT ` fst ` R"
     by (fastforce simp: image_iff)
   note * = derive_Cons_undef[OF this]
   from Cons.prems have "nt p \<inter> fst ` R = {}" by (auto simp: nt_Cons)
@@ -668,25 +668,25 @@ lemma deriven_append_undef:
 lemma fst_unwind_new: "fst ` unwind_new R A A' \<subseteq> {A'}"
   by (auto simp: unwind_new_def)
 
-lemma N_in_set_iff_nt: "N A \<in> set w \<longleftrightarrow> A \<in> nt w"
-  by (induction w, auto simp: nt_Cons split: symb.splits)
+lemma NT_in_set_iff_nt: "NT A \<in> set w \<longleftrightarrow> A \<in> nt w"
+  by (induction w, auto simp: nt_Cons split: sym.splits)
 
 lemma unwind_new_only_last:
   assumes A'R: "A' \<notin> Nt R"
-    and "unwind_new R A A' \<turnstile> [N A'] \<Rightarrow>(n) u"
-  shows "N A' \<notin> set u \<or> (\<exists>u'. u = u' @ [N A'] \<and> N A' \<notin> set u')"
+    and "unwind_new R A A' \<turnstile> [NT A'] \<Rightarrow>(n) u"
+  shows "NT A' \<notin> set u \<or> (\<exists>u'. u = u' @ [NT A'] \<and> NT A' \<notin> set u')"
   using assms(2)
 proof (induction n arbitrary: u)
   case 0
   then show ?case by auto
 next
   case (Suc n)
-  from Suc.prems obtain y where A'y: "unwind_new R A A' \<turnstile> [N A'] \<Rightarrow>(n) y"
+  from Suc.prems obtain y where A'y: "unwind_new R A A' \<turnstile> [NT A'] \<Rightarrow>(n) y"
     and yu: "unwind_new R A A' \<turnstile> y \<Rightarrow> u"
     by (auto simp: relpowp_Suc_right derive_singleton)
-  from yu have "N A' \<in> set y" by (auto simp: derive_iff unwind_new_def)
+  from yu have "NT A' \<in> set y" by (auto simp: derive_iff unwind_new_def)
   with Suc.IH[OF A'y]
-  obtain u' where [simp]: "y = u' @ [N A']" and A'u': "N A' \<notin> set u'" by auto
+  obtain u' where [simp]: "y = u' @ [NT A']" and A'u': "NT A' \<notin> set u'" by auto
   with yu have "\<exists>v. (A',v) \<in> unwind_new R A A' \<and> u = u' @ v"
     by (auto simp: derive_iff unwind_new_def append_eq_append_conv2
         append_eq_Cons_conv Cons_eq_append_conv)
@@ -696,9 +696,9 @@ qed
 
 lemma unwind_new_sound:
   assumes A'R: "A' \<notin> Nt R"
-    and "unwind_new R A A' \<turnstile> [N A'] \<Rightarrow>(n) vs"
-    and A'vs: "N A' \<notin> set vs"
-  shows "R \<turnstile> [N A] \<Rightarrow>* N A # vs"
+    and "unwind_new R A A' \<turnstile> [NT A'] \<Rightarrow>(n) vs"
+    and A'vs: "NT A' \<notin> set vs"
+  shows "R \<turnstile> [NT A] \<Rightarrow>* NT A # vs"
   using assms(2-)
 proof (induction n arbitrary: vs)
   case 0
@@ -706,34 +706,34 @@ proof (induction n arbitrary: vs)
 next
   let ?R' = "unwind_new R A A'"
   case (Suc n)
-  then obtain y where y: "?R' \<turnstile> [N A'] \<Rightarrow> y" 
+  then obtain y where y: "?R' \<turnstile> [NT A'] \<Rightarrow> y" 
     and yvs: "?R' \<turnstile> y \<Rightarrow>(n) vs" by (auto simp: relpowp_Suc_left)
   show ?case
   proof (cases n)
     case 0
     with yvs have [simp]: "y = vs" by auto
-    with Suc y have "\<exists>v. (A,N A # v) \<in> R \<and> y = v"
+    with Suc y have "\<exists>v. (A,NT A # v) \<in> R \<and> y = v"
       apply (simp add: unwind_new_def derive_singleton)
       by (auto simp: Nt_def split: prod.splits)
     then show ?thesis apply (intro r_into_rtranclp)
       by (auto simp: derive_singleton)
   next
     case (Suc m)
-    with yvs have "N A' \<in> set y"
+    with yvs have "NT A' \<in> set y"
       by (auto simp: relpowp_Suc_left unwind_new_def derive_iff)
     with A'R y obtain v
-      where AAv: "(A,N A # v) \<in> R" and [simp]: "y = v @ [N A']"
+      where AAv: "(A,NT A # v) \<in> R" and [simp]: "y = v @ [NT A']"
       by (auto simp: unwind_new_def derive_singleton Nt_def split: prod.splits)
-    from AAv A'R have A'v: "N A' \<notin> set v" by (auto simp: Nt_def)
+    from AAv A'R have A'v: "NT A' \<notin> set v" by (auto simp: Nt_def)
     with fst_unwind_new[of R A A']
-    have "nt v \<inter> fst ` ?R' = {}" by (auto simp: N_in_set_iff_nt)
+    have "nt v \<inter> fst ` ?R' = {}" by (auto simp: NT_in_set_iff_nt)
     from yvs[simplified] deriven_append_undef[OF this]
-    obtain w where [simp]: "vs = v @ w" and A'w: "?R' \<turnstile> [N A'] \<Rightarrow>(n) w"
+    obtain w where [simp]: "vs = v @ w" and A'w: "?R' \<turnstile> [NT A'] \<Rightarrow>(n) w"
       by blast
-    have "N A' \<notin> set w" using Suc.prems(2) by auto
+    have "NT A' \<notin> set w" using Suc.prems(2) by auto
     note Suc.IH[OF A'w this]
-    also have "R \<turnstile> N A # w \<Rightarrow> N A # vs"
-      using AAv derivel_N_Cons derivel_imp_derive by fastforce
+    also have "R \<turnstile> NT A # w \<Rightarrow> NT A # vs"
+      using AAv derivel_NT_Cons derivel_imp_derive by fastforce
     finally show ?thesis.
   qed
 qed
@@ -744,16 +744,16 @@ lemma right_loop_unwind:
   using assms
   by (auto simp: right_loop_def unwind_def unwind_old_def unwind_new_def Nt_def)
 
-lemma map_T_eq_map_T: "map T u = map T v \<longleftrightarrow> u = v"
-  by (metis list.inj_map_strong symb.inject(1))
+lemma map_Tm_eq_map_Tm: "map Tm u = map Tm v \<longleftrightarrow> u = v"
+  by (metis list.inj_map_strong sym.inject(2))
 
 lemma deriver_mono: "R \<subseteq> S \<Longrightarrow> deriver R \<le> deriver S"
   by (force simp: deriver.simps)
 
 lemma unwind_sound:
   assumes "unwind R A A' \<turnstile> u \<Rightarrow>r(n) v"
-    and "N A' \<notin> set u"
-    and "N A' \<notin> set v"
+    and "NT A' \<notin> set u"
+    and "NT A' \<notin> set v"
     and A'R: "A' \<notin> Nt R"
   shows "R \<turnstile> u \<Rightarrow>* v"
   using assms(1-3)
@@ -767,58 +767,58 @@ proof (induction n arbitrary: u v rule: less_induct)
     case [simp]: (Suc m)
     from less.prems obtain B w l r
       where BwR': "(B,w) \<in> unwind_old R A A'"
-        and [simp]: "u = l @ N B # map T r"
-        and m: "unwind R A A' \<turnstile> l @ w @ map T r \<Rightarrow>r(m) v"
+        and [simp]: "u = l @ NT B # map Tm r"
+        and m: "unwind R A A' \<turnstile> l @ w @ map Tm r \<Rightarrow>r(m) v"
       by (auto simp: relpowp_Suc_left append_eq_append_conv2 unwind_def unwind_new_def
           dest!:deriver_iff[THEN iffD1])
     from less.prems
-    have A'l: "N A' \<notin> set l" by auto
+    have A'l: "NT A' \<notin> set l" by auto
     show ?thesis
-    proof (cases "N A' \<in> set w")
+    proof (cases "NT A' \<in> set w")
       case True
       with BwR' A'R obtain w'
-        where [simp]: "B = A" "w = w' @ [N A']"
-          and Aw'R: "(A,w') \<in> R" and A'w': "N A' \<notin> set w'"
+        where [simp]: "B = A" "w = w' @ [NT A']"
+          and Aw'R: "(A,w') \<in> R" and A'w': "NT A' \<notin> set w'"
         by (auto simp: unwind_old_def Nt_def split: prod.splits)
-      from m[folded append_assoc, unfolded derivern_append_map_T]
-      obtain v' where v': "unwind R A A' \<turnstile> (l @ w') @ [N A'] \<Rightarrow>r(m) v'"
-        and [simp]: "v = v' @ map T r"
+      from m[folded append_assoc, unfolded derivern_append_map_Tm]
+      obtain v' where v': "unwind R A A' \<turnstile> (l @ w') @ [NT A'] \<Rightarrow>r(m) v'"
+        and [simp]: "v = v' @ map Tm r"
         by auto
       from less.prems have "\<not>ends_with A' v'" by (auto simp: ends_with_def)
       from extract_right_loop[OF v' this]
       obtain n1 n2 u' w'' where len: "n1 + n2 < m"
-        and n1: "right_loop (unwind R A A') A' \<turnstile> [N A'] \<Rightarrow>r(n1) u' @ [N A']"
+        and n1: "right_loop (unwind R A A') A' \<turnstile> [NT A'] \<Rightarrow>r(n1) u' @ [NT A']"
         and w'': "(A', w'') \<in> unwind R A A'" "\<not> ends_with A' w''"
         and n2: "unwind R A A' \<turnstile> (l @ w') @ u' @ w'' \<Rightarrow>r(n2) v'" by auto
       from w'' A'R have A'w''R: "(A',w'') \<in> unwind_new R A A'"
-        and A'w'': "N A' \<notin> set w''"
+        and A'w'': "NT A' \<notin> set w''"
         by (auto simp: unwind_def unwind_old_def unwind_new_def Nt_def ends_with_def)
       from n1 right_loop_unwind[OF A'R, THEN deriver_mono]
-      have n1: "unwind_new R A A' \<turnstile> [N A'] \<Rightarrow>r(n1) u' @ [N A']"
+      have n1: "unwind_new R A A' \<turnstile> [NT A'] \<Rightarrow>r(n1) u' @ [NT A']"
         apply (auto simp: le_fun_def)
         by (metis relpowp_mono)
       from unwind_new_only_last[OF A'R derivern_imp_deriven[OF n1]]
-      have A'u': "N A' \<notin> set u'" by auto
+      have A'u': "NT A' \<notin> set u'" by auto
       note n1
-      also have "unwind_new R A A' \<turnstile> u' @ [N A'] \<Rightarrow>r u' @ w''"
-        using A'w''R by (auto simp: deriver_snoc_N simp del: append_assoc)
-      finally have "unwind_new R A A' \<turnstile> [N A'] \<Rightarrow>(Suc n1) u' @ w''"
+      also have "unwind_new R A A' \<turnstile> u' @ [NT A'] \<Rightarrow>r u' @ w''"
+        using A'w''R by (auto simp: deriver_snoc_NT simp del: append_assoc)
+      finally have "unwind_new R A A' \<turnstile> [NT A'] \<Rightarrow>(Suc n1) u' @ w''"
         by (rule derivern_imp_deriven)
       from unwind_new_sound[OF A'R this] A'u' A'w' A'w''
-      have "R \<turnstile> [N A] \<Rightarrow>* N A # u' @ w''" by auto
+      have "R \<turnstile> [NT A] \<Rightarrow>* NT A # u' @ w''" by auto
       also have "R \<turnstile> \<dots> \<Rightarrow> w' @ u' @ w''" using Aw'R
-        by (auto intro!: derivel_imp_derive simp: derivel_N_Cons)
-      finally have "R \<turnstile> [N A] \<Rightarrow>* \<dots>".
+        by (auto intro!: derivel_imp_derive simp: derivel_NT_Cons)
+      finally have "R \<turnstile> [NT A] \<Rightarrow>* \<dots>".
       note derives_prepend[OF this]
       also from A'u' A'w' A'w'' less.prems(2-3) less.IH[OF _ n2] len
       have "R \<turnstile> l @ w' @ u' @ w'' \<Rightarrow>* v'" by auto
-      finally have "R \<turnstile> l @ [N A] \<Rightarrow>* v'".
+      finally have "R \<turnstile> l @ [NT A] \<Rightarrow>* v'".
       from derives_append[OF this]
       show ?thesis by simp
     next
       case False
       with BwR' have "(B,w) \<in> R" by (auto simp: unwind_old_def)
-      then have "R \<turnstile> u \<Rightarrow> l @ w @ map T r" by (auto simp: derive_iff)
+      then have "R \<turnstile> u \<Rightarrow> l @ w @ map Tm r" by (auto simp: derive_iff)
       also have "R \<turnstile> \<dots> \<Rightarrow>* v"
         apply (rule less.IH[OF _ m]) using A'R BwR' A'l False less.prems
         by (auto simp: Nt_def split:prod.splits)
@@ -828,20 +828,20 @@ proof (induction n arbitrary: u v rule: less_induct)
 qed
 
 lemma unwind_derives:
-  assumes "N A' \<notin> set u" and "A' \<notin> Nt R"
-  shows "unwind R A A' \<turnstile> u \<Rightarrow>* map T v \<longleftrightarrow> R \<turnstile> u \<Rightarrow>* map T v"
+  assumes "NT A' \<notin> set u" and "A' \<notin> Nt R"
+  shows "unwind R A A' \<turnstile> u \<Rightarrow>* map Tm v \<longleftrightarrow> R \<turnstile> u \<Rightarrow>* map Tm v"
     (is "?l \<longleftrightarrow> ?r")
 proof
   assume "?r"
-  then have "R \<turnstile> u \<Rightarrow>l* map T v" by (simp add: derivels_iff_derives)
-  then obtain n where "R \<turnstile> u \<Rightarrow>l(n) map T v"
+  then have "R \<turnstile> u \<Rightarrow>l* map Tm v" by (simp add: derivels_iff_derives)
+  then obtain n where "R \<turnstile> u \<Rightarrow>l(n) map Tm v"
     by (metis rtranclp_imp_relpowp)
   from unwind_complete[OF this]
   show "?l".
 next
   assume "?l"
-  then have "unwind R A A' \<turnstile> u \<Rightarrow>r* map T v" by (simp add: derivers_iff_derives)
-  then obtain n where "unwind R A A' \<turnstile> u \<Rightarrow>r(n) map T v"
+  then have "unwind R A A' \<turnstile> u \<Rightarrow>r* map Tm v" by (simp add: derivers_iff_derives)
+  then obtain n where "unwind R A A' \<turnstile> u \<Rightarrow>r(n) map Tm v"
     by (metis rtranclp_imp_relpowp)
   from unwind_sound[OF this ] assms
   show "?r" by auto
@@ -1222,7 +1222,7 @@ qed
 
 end
 
-value "unwind_expand_list [(1,[N 1 :: (int,int)symb, N 1])] [] 1 2"
+value "unwind_expand_list [(1,[N 1 :: (int,int)sym, N 1])] [] 1 2"
 
 theorem GNF:
 fixes R :: "('n,'t)prods" and new :: "'n set \<Rightarrow> 'n"
